comments and corrections

Triangle.thy
@@ -1,14 +1,22 @@
 theory Triangle
-imports GNF
+imports CFG
 begin
-(*
-Conjecture: fully expanded form is unique
-*)
 
-definition "hd_nts R = {B. \<exists>A w. (A,Nt B # w) \<in> R}"
-definition hd_nts_list :: "('n \<times> ('n, 't) sym list) list \<Rightarrow> 'n list" where
-"hd_nts_list R = [B. (A,Nt B # w) \<leftarrow> R]"
+(* The algorithm and an initial part of the proof. So far I have only tried to show that
+the result is of the right form (triangular). I have not tried to show that the language stays
+unchanged. That will be harder.*)
 
+(* The "real" functions are on sets, but there is often a list version as well.
+The list version is intended for quickcheck test only (because quickcheck cannot deal with set comprehension {x. ...}.
+Sometimes I have proved equivalence with the set version, but that is merely a sanity check.
+Testing with nitpick is possible also for sets, but seems to work less well than quickcheck *)
+
+definition "hdNts R = {B. \<exists>A w. (A,Nt B # w) \<in> R}"
+definition hdNts_list :: "('n \<times> ('n, 't) sym list) list \<Rightarrow> 'n list" where
+"hdNts_list R = [B. (A,Nt B # w) \<leftarrow> R]"
+
+text \<open>"Expand head: Replace all rules \<open>A \<rightarrow> B w\<close> where \<open>B \<in> Ss\<close> (\<open>Ss\<close> = solved Nts)
+by \<open>A \<rightarrow> v w\<close> where \<open>B \<rightarrow> v\<close>. Starting from the end of \<open>Ss\<close>\<close>
 fun exp_hd :: "'n \<Rightarrow> 'n list \<Rightarrow> ('n,'t)Prods \<Rightarrow> ('n,'t)Prods" where
 "exp_hd A [] R = R" |
 "exp_hd A (S#Ss) R =
@@ -16,11 +24,6 @@ fun exp_hd :: "'n \<Rightarrow> 'n list \<Rightarrow> ('n,'t)Prods \<Rightarrow>
       X = {(Al,Bw) \<in> R'. Al=A \<and> (\<exists>w. Bw = Nt S # w)};
       Y = {(A,v@w) |v w. \<exists>B. (A,Nt B # w) \<in> X \<and> (B,v) \<in> R'}
   in R' - X \<union> Y)"
-
-fun hd_in_As where
-"hd_in_As As [] = True" |
-"hd_in_As As (Tm _ # _) = True" |
-"hd_in_As As (Nt B # _) = (B \<in> set As)"
 
 fun exp_hd_list :: "'n \<Rightarrow> 'n list \<Rightarrow> ('n,'t)prod list \<Rightarrow> ('n,'t)prod list" where
 "exp_hd_list A [] R = R" |
@@ -30,13 +33,14 @@ fun exp_hd_list :: "'n \<Rightarrow> 'n list \<Rightarrow> ('n,'t)prod list \<Ri
   [(B,w) \<leftarrow> R'. (B,w) \<notin> set X] @
   [(A,v@w). (_,Nt B # w) \<leftarrow> X, (C,v) \<leftarrow> R', B = C])"
 
-value "exp_hd_list (1::int)[3,2][(1, [Nt 2]::(int,int)sym list)]"
-
+value "exp_hd_list (1::int) [2,3] [(1, [Nt 2,Tm 0]::(int,int)sym list), (2,[Nt 3]), (3,[Tm 1])]"
+value "exp_hd_list (1::int) [3,2] [(1, [Nt 2]::(int,int)sym list)]"
 
 lemma "set(exp_hd_list A As R) = exp_hd A As (set R)"
-nitpick
+(*nitpick*)
 oops
 
+text \<open>Remove left-recursive rules\<close>
 definition rm_lrec ::  "'n \<Rightarrow> ('n,'t)Prods \<Rightarrow> ('n,'t)Prods" where
 "rm_lrec A R = R - {(A,Nt A # v)|v. True}"
 
@@ -57,8 +61,9 @@ definition rm_lrec_list ::  "'n \<Rightarrow> ('n,'t)prod list \<Rightarrow> ('n
 lemma "set(rm_lrec_list A R) = rm_lrec A (set R)"
 by(auto simp: rm_lrec_list_def rm_lrec_def hd_not_NA_list)
 
-(* split into A \<rightarrow> u | Av; retain A \<rightarrow> u; add A \<rightarrow> uA', A' \<rightarrow> v | vA' *)
-
+text \<open>Conversion from left-recursion to right-recursion:
+Split \<open>A\<close>-rules into \<open>A \<rightarrow> u\<close> and \<open>A \<rightarrow> A v\<close>.
+Keep \<open>A \<rightarrow> u\<close> but replace \<open>A \<rightarrow> A v\<close> by \<open>A \<rightarrow> u A'\<close>, \<open>A' \<rightarrow> v\<close>, \<open>A' \<rightarrow> v A'\<close>:\<close>
 definition rrec_of_lrec ::  "'n \<Rightarrow> 'n \<Rightarrow> ('n,'t)Prods \<Rightarrow> ('n,'t)Prods" where
 "rrec_of_lrec A A' R =
   (let V = {v. (A,Nt A # v) \<in> R \<and> v \<noteq> []};
@@ -70,41 +75,33 @@ definition rrec_of_lrec_list ::  "'n \<Rightarrow> 'n \<Rightarrow> ('n,'t)prod 
   (let V = [v. (Al,Nt Ar # v) \<leftarrow> R, Al=A, Ar=A, v \<noteq> []];
        U = [u. (Al,u) \<leftarrow> R, Al=A, hd_not_NA_list A u]
   in [(A,u). u \<leftarrow> U] @ [(A,u@[Nt A']). u \<leftarrow> U] @ [(A',v). v \<leftarrow> V] @ [(A',v @ [Nt A']). v \<leftarrow>V])"
-(*
-lemma "set(rrec_of_lrec_list A A' R) = rrec_of_lrec A A' (set R)"
-apply(auto simp: rrec_of_lrec_def rrec_of_lrec_list_def Let_def image_def hd_not_NA_list)
-apply blast
-  apply blast
-  apply blast
-apply(auto simp: rrec_of_lrec_def rrec_of_lrec_list_def Let_def image_def hd_not_NA_list
-  split: prod.splits if_splits intro:)[]
-  apply (metis list.set_intros(1))
-apply(auto simp: rrec_of_lrec_def rrec_of_lrec_list_def Let_def image_def hd_not_NA_list
-  split: prod.splits list.splits symb.splits if_splits)
-  apply (metis list.set_intros(1))
-apply (smt (verit) Pair_inject list.distinct(1) list.set_intros(1) list.simps(1) symb.simps(2,4)) 
-apply (smt (verit) Pair_inject list.distinct(1) list.set_intros(1) list.simps(1) symb.simps(2,4))
-  apply (metis list.set_intros(1))
-  by (metis list.set_intros(1))
-*)
+
+text \<open>Dealing with ("solving") Nt A. The new Nt A' is also given as a parameter.\<close>
 definition solve_lrec ::  "'n \<Rightarrow> 'n \<Rightarrow> ('n,'t)Prods \<Rightarrow> ('n,'t)Prods" where
 "solve_lrec A A' R = rm_lrec A R \<union> rrec_of_lrec A A' R"
 
 definition solve_lrec_list ::  "'n \<Rightarrow> 'n \<Rightarrow> ('n,'t)prod list \<Rightarrow> ('n,'t)prod list" where
 "solve_lrec_list A A' R = rm_lrec_list A R @ rrec_of_lrec_list A A' R"
 
+text \<open>Put \<open>R\<close> into triangular form wrt \<open>As\<close> (using the new Nts \<open>As'\<close>).
+That means that \<open>As\<close> are the Nts that still have to be solved.
+In each step \<open>A#As\<close>, first the remaining \<open>As\<close> are solved, then \<open>A\<close> is solved.
+This should mean that in the result of the outermost \<open>exp_hd A As\<close>, \<open>A\<close> only depends on \<open>A\<close>,
+i.e. the \<open>A\<close> rules in the result of \<open>solve_lrec A A'\<close> are already in GNF. More precisely:
+the result should be in triangular form.\<close>
 fun solve_tri where
 "solve_tri [] _ R = R" |
-"solve_tri (A#As) (A'#As') R = solve_tri As As' (solve_lrec A A' (exp_hd A As R))"
+"solve_tri (A#As) (A'#As') R = solve_lrec A A' (exp_hd A As (solve_tri As As' R))"
 
 fun solve_tri_list where
 "solve_tri_list [] _ R = R" |
-"solve_tri_list (A#As) (A'#As') R = solve_tri_list As As' (solve_lrec_list A A' (exp_hd_list A As R))"
+"solve_tri_list (A#As) (A'#As') R = solve_lrec_list A A' (exp_hd_list A As (solve_tri_list As As' R))"
 
 lemma "set(solve_tri_list As As' R) = solve_tri As As' (set R)"
-nitpick
+(*nitpick*)
 oops
 
+text \<open>\<open>A\<close> depends on \<open>B\<close> if there is a rule \<open>A \<rightarrow> B w\<close>:\<close>
 definition dep_on :: "('n,'t) Prods \<Rightarrow> 'n \<Rightarrow> 'n set" where
 "dep_on R A = {B. \<exists>w. (A,Nt B # w) \<in> R}"
 
@@ -114,17 +111,19 @@ definition dep_on_list :: "('n,'t) prod list \<Rightarrow> 'n \<Rightarrow> 'n l
 lemma "set(dep_on_list R A) = dep_on (set R) A"
 by(auto simp: dep_on_def dep_on_list_def)
 
+text \<open>Triangular form wrt \<open>[A1,\<dots>,An]\<close> means that \<open>Ai\<close> must not depend on \<open>Ai, \<dots>, An\<close>.
+In particular: \<open>A0\<close> does not depend on any \<open>Ai\<close>: its rules are already in GNF.
+Therefore one can convert a triangular form into GNF by backwards substitution:
+the rules for \<open>Ai\<close> are used to expand the heads of all \<open>A(i+1),\<dots>,An\<close> rules,
+starting with \<open>A0\<close>.\<close>
+
 fun triangular :: "'n list \<Rightarrow> ('n \<times> ('n, 't) sym list) set \<Rightarrow> bool" where
 "triangular [] R = True" |
 "triangular (A#As) R = (dep_on R A \<inter> ({A} \<union> set As) = {} \<and> triangular As R)"
-(*
-fun triangular :: "'n list \<Rightarrow> 'n set \<Rightarrow> ('n \<times> ('n, 't) symb list) set \<Rightarrow> bool" where
-"triangular [] S R = True" |
-"triangular (A#As) S R = (dep_on R A \<inter> ({A} \<union> S) = {} \<and> triangular As ({A} \<union> S) R)"
-*)
-fun triangular_list :: "'a list \<Rightarrow> 'a set \<Rightarrow> ('a \<times> ('a, 'b) sym list) list \<Rightarrow> bool" where
-"triangular_list [] S R = True" |
-"triangular_list (A#As) S R = (set(dep_on_list R A) \<inter> ({A} \<union> S) = {} \<and> triangular_list As ({A} \<union> S) R)"
+
+fun triangular_list :: "'a list \<Rightarrow> ('a \<times> ('a, 'b) sym list) list \<Rightarrow> bool" where
+"triangular_list [] R = True" |
+"triangular_list (A#As) R = (set(dep_on_list R A) \<inter> ({A} \<union> set As) = {} \<and> triangular_list As R)"
 
 lemma exp_hd_preserves: "(A, Nt S # w) \<in> R \<Longrightarrow> S \<notin> set Ss \<Longrightarrow> (A, Nt S # w) \<in> exp_hd A Ss R"
 proof(induction A Ss R rule: exp_hd.induct)
@@ -136,20 +135,17 @@ next
     by(auto simp: Let_def)
 qed
 
+(* Should be true. Easy induction? *)
 lemma exp_hd_preserves_neq: "B \<noteq> A \<Longrightarrow> (B,w) \<in> exp_hd A Ss R \<longleftrightarrow> (B,w) \<in> R"
 sorry
 
+(* True! Later *)
 lemma Eps_free_exp_hd: "Eps_free R \<Longrightarrow> Eps_free (exp_hd A Ss R)"
 sorry
 
-(*
-lemma dep_on_exp_hd:
-  "\<lbrakk> Eps_free_list R; triangular_list (rev Bs) S R; distinct Bs; A \<notin> set Bs \<rbrakk>
- \<Longrightarrow> set(dep_on_list (exp_hd_list A Bs R) A) \<subseteq> (set(dep_on_list R A) \<union> (\<Union>B\<in>set Bs. set(dep_on_list R B))) - set Bs"
-quickcheck
-value "exp_hd_list (1::int)[3][(1, [N 2]::(int,int)symb list),(2,[N 3])]"
-oops
-*)
+text \<open>Let \<open>R\<close> be epsilon-free and in triangular form wrt \<open>Bs\<close>.
+After \<open>exp_hd A Bs R\<close>, \<open>A\<close> depends only on what \<open>A\<close> depended on before or
+what one of the \<open>B \<in> Bs\<close> depends on, but \<open>A\<close> does not depend on the \<open>Bs\<close>:\<close>
 lemma dep_on_exp_hd:
   "\<lbrakk> Eps_free R; triangular Bs R; distinct Bs; A \<notin> set Bs \<rbrakk>
  \<Longrightarrow> dep_on (exp_hd A Bs R) A \<subseteq> (dep_on R A \<union> (\<Union>B\<in>set Bs. dep_on R B)) - set Bs"
@@ -162,45 +158,27 @@ next
     by(fastforce simp add: Let_def dep_on_def Cons_eq_append_conv Eps_free_exp_hd Eps_free_Nil exp_hd_preserves_neq set_eq_iff)
 qed
 
+(* ? *)
 lemma dep_on_exp_hd_step:
   "\<lbrakk> dep_on R B \<inter> ({B} \<union> set Ts) = {}; distinct (B#Ts); A \<notin> set(B#Ts) \<rbrakk> \<Longrightarrow> dep_on (exp_hd A (B#Ts) R) A = dep_on(exp_hd A Ts R) A - {B}"
 apply(simp add: Let_def)
-sorry
+oops
 
+(* ? *)
 lemma "\<lbrakk> Eps_free R; A \<notin> set Ts \<union> S; dep_on R A \<inter> S = {} ; triangular Ts R; distinct Ts \<rbrakk> \<Longrightarrow> dep_on (exp_hd A Ts R) A \<inter> (set Ts \<union> S) = {}"
 (*nitpick*)
-proof(induction A Ts R arbitrary: S rule: exp_hd.induct)
-  case (1 A R)
-  then show ?case by auto
-next
-  case (2 A T Ts R)
-  then show ?case
-apply(simp add: Let_def del: exp_hd.simps)
-apply safe
-apply (clarsimp simp add: dep_on_def Let_def)
-apply(erule disjE)
-apply safe[]
-apply (auto simp: exp_hd_preserves)[]
-apply safe[]
-apply(simp add: Cons_eq_append_conv)
-apply safe[]
-    apply (meson Eps_free_Nil Eps_free_exp_hd)
-apply(simp add: exp_hd_preserves_neq)
-apply (clarsimp simp del: exp_hd.simps)
-apply(subst (asm) dep_on_exp_hd_step)
-apply simp
-apply(erule disjE)
-apply safe[]
-apply(erule_tac x="insert T S" in meta_allE)
-apply(auto)[]
+oops
 
- sorry
-qed
-nitpick
+lemma "\<lbrakk> eps_free R; length As \<le> length As'; distinct(As @ As'); nts R \<subseteq> set As \<rbrakk>
+  \<Longrightarrow> triangular_list As (solve_tri_list As As' R)"
+(* quickcheck  no counterexample found - not clear if that means much here *)
+oops
 
-lemma "\<lbrakk> length As \<le> length As'; distinct(As @ As'); Nt R \<subseteq> set As \<rbrakk>
+(* This is the first key result we need: \<open>solve_tri\<close> produces a triangular form *)
+lemma triangular_solve_tri:  "\<lbrakk> Eps_free R; length As \<le> length As'; distinct(As @ As'); Nts R \<subseteq> set As \<rbrakk>
   \<Longrightarrow> triangular As (solve_tri As As' R)"
-nitpick
+(* nitpick  no counterexample found - not clear if that means much here *)
+
 oops
 
 lemma Eps_free_exp_hd[simp]: "Eps_free (exp_hd A As R) = Eps_free R"
@@ -260,15 +238,15 @@ quickcheck
 oops
 
 value "dep_on_list [(1,[T 5]::(int,int)symb list)] 1 []"
-value "hd_nts_list[(1,[T 5]::(int,int)symb list)]"
+value "hdNts_list[(1,[T 5]::(int,int)symb list)]"
 value "solve_tri_list [1] [2] [(1,[N 1, N 1]::(int,int)symb list)]"
 
-lemma hd_nts_exp_hd: "Eps_free R \<Longrightarrow> hd_nts (exp_hd A As R) \<subseteq> hd_nts R"
-by(fastforce simp: hd_nts_def exp_hd_def dest: Eps_freeE_Cons)
+lemma hdNts_exp_hd: "Eps_free R \<Longrightarrow> hdNts (exp_hd A As R) \<subseteq> hdNts R"
+by(fastforce simp: hdNts_def exp_hd_def dest: Eps_freeE_Cons)
 
 (* used? *)
-lemma hd_nts_solve_lrec: "hd_nts (solve_lrec A A' R) \<subseteq> Nt R"
-by(auto simp: hd_nts_def solve_lrec_def rrec_of_lrec_def rm_lrec_def Cons_eq_append_conv
+lemma hdNts_solve_lrec: "hdNts (solve_lrec A A' R) \<subseteq> Nt R"
+by(auto simp: hdNts_def solve_lrec_def rrec_of_lrec_def rm_lrec_def Cons_eq_append_conv
    dest: Eps_freeE_Cons dest: hd_in_Nt hd2_in_Nt)
 
 lemma Eps_free_Un: "Eps_free (R \<union> S) = (Eps_free R \<and> Eps_free S)"
@@ -289,27 +267,27 @@ by(auto simp: solve_lrec_def Eps_free_Un)
 lemma Eps_free_exp_hd[simp]: "Eps_free R \<Longrightarrow> Eps_free (exp_hd A As R)"
 by(auto simp: exp_hd_def Eps_free_def split: prod.splits)
 
-lemma hd_nts_exp_hd_Un: "\<lbrakk> Eps_free R; A' \<notin> Nt R; A' \<notin> hd_nts RA'; \<forall>(A,w) \<in> RA'. A=A' \<rbrakk>
- \<Longrightarrow> hd_nts (exp_hd A' {} (R \<union> RA')) \<subseteq> hd_nts R"
-by(auto simp add: exp_hd_def hd_nts_def Nt_def subset_iff Eps_free_def Cons_eq_append_conv split: prod.splits)
+lemma hdNts_exp_hd_Un: "\<lbrakk> Eps_free R; A' \<notin> Nt R; A' \<notin> hdNts RA'; \<forall>(A,w) \<in> RA'. A=A' \<rbrakk>
+ \<Longrightarrow> hdNts (exp_hd A' {} (R \<union> RA')) \<subseteq> hdNts R"
+by(auto simp add: exp_hd_def hdNts_def Nt_def subset_iff Eps_free_def Cons_eq_append_conv split: prod.splits)
 
-corollary hd_nts_exp_hd_solve_lrec: "\<comment>\<open>\<lbrakk> Eps_free R; A' \<notin> Nt R; A' \<notin> hd_nts RA'; \<forall>(A,w) \<in> RA'. A=A' \<rbrakk>
- \<Longrightarrow>\<close> hd_nts (exp_hd A' {} (solve_lrec A A' R)) \<subseteq> hd_nts R"
+corollary hdNts_exp_hd_solve_lrec: "\<comment>\<open>\<lbrakk> Eps_free R; A' \<notin> Nt R; A' \<notin> hdNts RA'; \<forall>(A,w) \<in> RA'. A=A' \<rbrakk>
+ \<Longrightarrow>\<close> hdNts (exp_hd A' {} (solve_lrec A A' R)) \<subseteq> hdNts R"
 unfolding solve_lrec_def
 sorry(*
-apply(rule hd_nts_exp_hd_Un)
-by(auto simp add: exp_hd_def hd_nts_def Nt_def subset_iff Eps_free_def Cons_eq_append_conv split: prod.splits)
+apply(rule hdNts_exp_hd_Un)
+by(auto simp add: exp_hd_def hdNts_def Nt_def subset_iff Eps_free_def Cons_eq_append_conv split: prod.splits)
 *)
-lemma "\<lbrakk> Eps_free R; length As = length As' \<rbrakk> \<Longrightarrow> hd_nts (solve_tri As As' R) \<subseteq> hd_nts R - set As"
+lemma "\<lbrakk> Eps_free R; length As = length As' \<rbrakk> \<Longrightarrow> hdNts (solve_tri As As' R) \<subseteq> hdNts R - set As"
 proof(induction As As' R rule: solve_tri.induct)
   case (2 A As A' As' R)
   then show ?case
- using hd_nts_exp_hd[of R A "set As"]
+ using hdNts_exp_hd[of R A "set As"]
 apply (simp)
 apply (simp add: solve_lrec_def)
 apply (auto simp add: Eps_free_UN)
 unfolding solve_lrec_def Let_def
-    using hd_nts_solve_lrec  by fas tforce
+    using hdNts_solve_lrec  by fas tforce
 qed auto
 
 apply simp
@@ -318,9 +296,9 @@ apply(rule subset_trans)
 apply(erule meta_allE)
 apply(erule meta_mp)
   apply (simp add: Eps_free_solve_lrec Eps_free_exp_hd)
-  using hd_nts_solve_lrec ldep_on_exp_hd by fa stforce
+  using hdNts_solve_lrec ldep_on_exp_hd by fa stforce
 
-lemma "Eps_free R \<Longrightarrow> hd_nts (solve_tri As R) \<subseteq> hd_nts R - set As"
+lemma "Eps_free R \<Longrightarrow> hdNts (solve_tri As R) \<subseteq> hdNts R - set As"
 apply(induction As arbitrary: R)
 apply simp
 apply simp
@@ -328,9 +306,9 @@ apply(rule subset_trans)
 apply(erule meta_allE)
 apply(erule meta_mp)
   apply (simp add: Eps_free_solve_lrec Eps_free_exp_hd)
-  using hd_nts_solve_lrec ldep_on_exp_hd by fastforce
+  using hdNts_solve_lrec ldep_on_exp_hd by fastforce
 
-  by (metis bot.extremum_uniqueI solve_lrec_def empty_Diff Eps_free_solve_lrec hd_nts_solve_lrec subsetI subset_Diff_insert)
+  by (metis bot.extremum_uniqueI solve_lrec_def empty_Diff Eps_free_solve_lrec hdNts_solve_lrec subsetI subset_Diff_insert)
 
 type_synonym 'a ix = "'a * nat"
 
